---  
publish: true  
---  
Sometimes it's easier to modify an equation so it becomes a full quadradic equation.  
  
Take the following:  
  
$$  
x^2+8x+11=0  
$$  
  
As it is this is not factorable, and while you can use quadratic method instead, you can force it to be factorable!  
  
You can do this whenever the b term is *even*, this will not work if b term is *odd*.  
  
First, move the c term to the other side of the equation, then multiply the middle term by 2 and add it to both sides of the equation  
$$  
\begin{align}  
x^2+8x+16 &=-11+16  \\  
\color{blue}x^2+8x+16&=\color{blue}5  
\end{align}  
$$  
Now, because the equation is in the format of $x^2+bx+2(b)=c$, we can rewrite it as the following!  
$$  
(x+4)^2=5  
$$  
Now you can use the square root property!  
  
$$  
\begin{align}  
\sqrt{ (x+4)^2 }&=\pm\sqrt{ 5 }\\  
x+4&=\pm \sqrt{ 5 } \\  
\color{blue}x&=\color{blue}-4\pm \sqrt{ 5 }  
\end{align}  
$$